newtype uint64 = fromNum nat
Replace the entire machine numbers model with a single type, uint64,
which is a wrapper around a nat. To retain some level of soundness,
during extraction we'll do overflow checks and throw an exception (so at
least the program doesn't execute doing something wrong).

It does seem like uint64s are good enough for our purposes; uint32s are
fairly similar in performance and size, and the one use case for uint16s
was for encoding value lengths. If we want that back, we can always
provide a function to encode/decode a bounded u64 in two bytes.

src/Database/BinaryEncoding.v
@@ -1,6 +1,6 @@
 From Coq Require Import FunctionalExtensionality.
 From Coq Require Import Program.Wf.
-From Coq Require Import NArith.NArith.
+From Coq Require Import micromega.Lia.
 From RecoveryRefinement Require Import Helpers.MachinePrimitives.
 From RecoveryRefinement Require Import Database.Common.
 
@@ -9,14 +9,14 @@ From Tactical Require Import ProofAutomation.
 From Classes Require Import EqualDec.
 Import EqualDecNotation.
 
-Import BSNotations.
+Import BSNotations UIntNotations.
 
 Definition Decoder T := ByteString -> option (T * uint64).
 
 Definition decodeBind T1 T2 (dec1: Decoder T1) (dec2: T1 -> Decoder T2) : Decoder T2 :=
   fun bs => match dec1 bs with
          | Some (v1, n) => match dec2 v1 (BS.drop n bs) with
-                          | Some (v2, n2) => Some (v2, intPlus n n2)
+                          | Some (v2, n2) => Some (v2, (n + n2)%u64)
                           | None => None
                           end
          | None => None
@@ -36,19 +36,19 @@ Proof.
 Abort.
 
 Definition decodeRet T (v:T) : Decoder T :=
-  fun _ => Some (v, int_val0).
+  fun _ => Some (v, fromNum 0).
 
 Definition decodeFail {T} : Decoder T :=
   fun _ => None.
 
 Definition decodeFinished : Decoder unit :=
-  fun bs => match intCmp (BS.length bs) int_val0 with
+  fun bs => match compare (BS.length bs) 0 with
          | Gt => None
-         | _ => Some (tt, int_val0)
+         | _ => Some (tt, 0%u64)
          end.
 
 Definition decodeFixed (n:uint64) : Decoder ByteString :=
-  fun bs => match intCmp (BS.length bs) n with
+  fun bs => match compare (BS.length bs) n with
          | Gt => None
          | _ => Some (BS.take n bs, n)
          end.
@@ -92,32 +92,32 @@ Proof.
                  ret (v1, v2); |}.
 Defined.
 
-Instance uint_fmt `{enc:@UIntEncoding bits good intTy int} : Encodable intTy :=
+Instance uint64_fmt : Encodable uint64 :=
   {| encode := encodeLE;
     decode := fun bs =>
                 match decodeLE bs with
-                | Some x => Some (x, fromNum numBytes)
+                | Some x => Some (x, fromNum 8)
                 | None => None
                 end; |}.
 
-Record Array16 := array16 { getBytes :> ByteString }.
+Record Array64 := array64 { getBytes :> ByteString }.
 
-Instance array16_fmt : Encodable Array16.
+Instance array64_fmt : Encodable Array64.
 Proof.
-  refine {| encode := fun (bs:Array16) =>
-              array16 (encode (as_uint uint16 (BS.length bs)) ++ bs);
+  refine {| encode := fun (bs:Array64) =>
+              array64 (encode (BS.length bs) ++ bs);
             decode :=
-              l <- decode uint16;;
-                array16 <$> decodeFixed (as_uint uint64 l); |}.
+              l <- decode uint64;;
+                array64 <$> decodeFixed l; |}.
 Defined.
 
 Instance entry_fmt : Encodable Entry.t.
 Proof.
   refine {| encode :=
-              fun e => encode e.(Entry.key) ++ encode (array16 e.(Entry.value));
+              fun e => encode e.(Entry.key) ++ encode (array64 e.(Entry.value));
             decode :=
               key <- decode uint64;;
-            value <- getBytes <$> decode Array16;;
+            value <- getBytes <$> decode Array64;;
             ret (Entry.mk key value); |}.
 Defined.
 
@@ -130,9 +130,9 @@ Fixpoint encode_list T (enc: T -> ByteString) (l: list T) : ByteString :=
 Program Fixpoint decode_list T (dec: Decoder T) (bs:ByteString)
         {measure (toNum (BS.length bs)) lt} : option (list T * uint64) :=
   if bs == BS.empty
-  then Some (nil, int_val0)
+  then Some (nil, 0)
   else match dec bs with
-       | Some (x, n) => if intCmp n int_val0 == Eq then None else
+       | Some (x, n) => if n == 0 then None else
                          match decode_list dec (BS.drop n bs) with
                          | Some (x', n') => Some (cons x x', n')
                          | None => None
@@ -142,9 +142,15 @@ Program Fixpoint decode_list T (dec: Decoder T) (bs:ByteString)
 Next Obligation.
   intros.
   rewrite drop_length.
-  (* TODO: need a lot more assumptions about uint64's to prove this
-  inequality *)
-Admitted.
+  simpl.
+  destruct n as [n]; simpl in *.
+  destruct bs as [bs]; simpl in *.
+  u64_cleanup.
+  assert (length bs > 0).
+  destruct bs; simpl in *; try lia.
+  exfalso; eauto.
+  lia.
+Qed.
 Next Obligation.
   apply measure_wf.
   apply Wf_nat.lt_wf.
@@ -167,7 +173,7 @@ Proof.
                     ++ encode h.(SliceHandle.length);
             decode :=
               offset <- decode uint64;;
-            length <- decode uint32;;
+            length <- decode uint64;;
             ret (SliceHandle.mk offset length);
          |}.
 Defined.
