src/Helpers/ExtrMachinePrimitives.v
@@ -1,5 +1,6 @@
 From Coq Require Import Extraction.
 From Coq Require Import ExtrHaskellBasic.
+From Coq Require Import ExtrHaskellNatInteger.
 
 From RecoveryRefinement Require Import Helpers.MachinePrimitives.
 
@@ -8,21 +9,17 @@ to a fiximports.py script *)
 
 Extraction Language Haskell.
 
-Extract Inlined Constant uint64 => "Data.Word.Word64".
-Extract Inlined Constant uint32 => "Data.Word.Word32".
-Extract Inlined Constant uint16 => "Data.Word.Word16".
-Extract Inlined Constant uint8  => "Data.Word.Word8".
+Extract Inductive uint64 => "Data.Word.Word64" ["fromIntegral"].
+(* fromNum might be used by constants, but there shouldn't be any use case for
+toNum *)
+Extract Inlined Constant toNum => "undefined".
 
 Extract Inductive comparison => "Prelude.Ordering" ["Prelude.EQ" "Prelude.LT" "Prelude.GT"].
 
-(* TODO: for now, left toNum/fromNum as undefined, but could theoretically
-extract to fromIntegral and convert to Integer (instead of nat) *)
-Extract Constant uint64_uint => "Build_UInt undefined undefined (+) (-) compare".
-Extract Constant uint32_uint => "Build_UInt undefined undefined (+) (-) compare".
-Extract Constant uint16_uint => "Build_UInt undefined undefined (+) (-) compare".
-Extract Constant uint8_uint  => "Build_UInt undefined undefined (+) (-) compare".
-
-(* TODO: need to axiomatize conversions in order to extract them to reasonable things, rather than going through Integer *)
+(* TODO: need checked versions of these *)
+Extract Inlined Constant add => "(+)".
+Extract Inlined Constant sub => "(-)".
+Extract Inlined Constant compare => "compare".
 
 (* extract these to a real type, but don't provide any constructor *)
 Extract Inductive ByteString => "Data.ByteString.ByteString" ["undefined"].
